Make the [language] interface more abstract
Move head_step & low-level property on evaluation contexts "under" the
abstraction barrier of the language interface. The goal is to make
[language] closer to [mlanguage], ando only expose properties that we
really need for the rest of the setup, in order to make it easier to
make change to the individual languages' semantics.

We also get rid of [wp_bind_inv] (that we did not use), which allows
us to stop proving some tricky properties (that might not be very
robust wrt future language extensions).

theories/c_lang/lang.v
@@ -6,6 +6,12 @@ From iris.prelude Require Import options.
 From melocoton Require Import stdpp_extra language_commons.
 From melocoton.c_interface Require Import defs.
 
+(* Engineering note: definitions and lemmas defined as [Local] correspond to
+   fields of [LanguageMixin] that thus get re-exported as generic functions on a
+   [language]. We define them as local to avoid the ml_lang-specific name
+   clashing with the generic name, and always pick the generic name.
+*)
+
 Declare Scope c_expr_scope.
 Delimit Scope c_expr_scope with CE.
 
@@ -188,30 +194,16 @@ Definition arity (F : function) := match F with Fun b e => length b end.
 
 Notation of_val := Val (only parsing).
 
-Definition of_class_C (e : mixin_expr_class) : expr :=
+Local Definition to_val (e : expr) : option val :=
   match e with
-  | ExprVal v => Val v
-  | ExprCall vf vl => FunCall (Val $ LitV $ LitFunPtr vf) (map Val vl)
-  end.
-
-#[local] Notation omap f x := (match x with Some v => f v | None => None end).
-
-Fixpoint unmap_val el :=
-  match el with
-  | Val v::er => omap (fun vr => Some (v::vr)) (unmap_val er)
-  | [] => Some nil
+  | Val v => Some v
   | _ => None
   end.
 
-Definition to_class_C (e : expr) : option mixin_expr_class :=
-  match e with
-  | Val v => Some (ExprVal v)
-  | FunCall (Val (LitV (LitFunPtr vf))) el => omap (fun l => Some (ExprCall vf l)) (unmap_val el)
-  | _ => None
-  end.
-
-Local Notation to_val e :=
-  (match to_class_C e with Some (ExprVal v) => Some v | _ => None end).
+Local Lemma to_of_val v : to_val (of_val v) = Some v.
+Proof. done. Qed.
+Local Lemma of_to_val e v : to_val e = Some v → of_val v = e.
+Proof. destruct e; inversion 1; done. Qed.
 
 (** Equality and other typeclass stuff *)
 Global Instance of_val_inj : Inj (=) (=) of_val.
@@ -252,9 +244,6 @@ Proof.
      | _, _ => right _
      end); try (clear gol); (clear go; abstract intuition congruence).
 Defined.
-
-Class program := prog : gmap string function.
-
 
 Global Instance un_op_finite : Countable un_op.
 Proof.
@@ -456,7 +445,7 @@ Fixpoint zip_args (an : list binder) (av : list val) : option (gmap string val) 
 Definition apply_function (f:function) (av : list val) := match f with Fun an e =>
     match (zip_args an av) with Some σ => Some (subst_all σ e) | _ => None end end.
 
-Inductive head_step (p : program) : expr → c_state → expr → c_state → Prop :=
+Inductive head_step (p : gmap string function) : expr → c_state → expr → c_state → Prop :=
   | LetS x v1 e2 ee σ :
      ee = subst' x v1 e2 ->
      head_step p (Let x (Val v1) e2) σ ee σ
@@ -491,22 +480,59 @@ Inductive head_step (p : program) : expr → c_state → expr → c_state → Pr
   | WhileS e1 e2 σ :
      head_step p (While e1 e2) σ (If e1 (Let BAnon e2 (While e1 e2)) (Val $ LitV $ LitInt 0)) σ
   | FunCallS s va args res e σ :
-     (p : gmap string function) !! s = Some (Fun args e) →
+     p !! s = Some (Fun args e) →
      apply_function (Fun args e) va = Some res →
      head_step p (FunCall (Val $ LitV $ LitFunPtr s) (map Val va)) σ res σ.
 
+Definition head_reducible (p : gmap _ _) (e : expr) (σ : c_state) :=
+  ∃ e' σ', head_step p e σ e' σ'.
+
+Inductive prim_step p : expr → c_state → expr → c_state → Prop :=
+  Prim_step K e1 e2 σ1 σ2 e1' e2' :
+    e1 = fill K e1' → e2 = fill K e2' →
+    head_step p e1' σ1 e2' σ2 → prim_step p e1 σ1 e2 σ2.
+
+(** External calls *)
+
+Local Definition of_call fn (vs: list val) : expr :=
+   FunCall (Val $ LitV $ LitFunPtr fn) (map Val vs).
+
+Local Definition is_call e fn vs K :=
+  e = fill K (of_call fn vs).
 
 (** Basic properties about the language *)
+
+Lemma alloc_fresh p n σ :
+  let l := fresh_locs (dom σ) in
+  (0 < n)%Z →
+  head_step p (Malloc ((Val $ LitV $ LitInt $ n))) σ
+            (Val $ LitV $ LitLoc l) (state_init_heap l n Uninitialized σ).
+Proof.
+  intros.
+  apply MallocS; first done.
+  intros. apply not_elem_of_dom.
+  by apply fresh_locs_fresh.
+Qed.
+
 Global Instance fill_item_inj Ki : Inj (=) (=) (fill_item Ki).
 Proof. induction Ki; intros ???; simplify_eq/=; auto with f_equal. Qed.
+
+Lemma fill_comp_item k K e : fill (k :: K) e = fill K (fill_item k e).
+Proof. reflexivity. Qed.
+
+Global Instance fill_inj K : Inj (=) (=) (fill K).
+Proof.
+  intros e1 e2.
+  induction K as [|Ki K IH] in e1, e2 |- *; rewrite /Inj; first done.
+  rewrite !fill_comp_item. by intros ?%IH%fill_item_inj.
+Qed.
 
 Lemma val_head_stuck p e1 σ1 e2 σ2 : head_step p e1 σ1 e2 σ2 → to_val e1 = None.
 Proof.
   inversion 1; simplify_eq; try done.
-  cbn. repeat (case_match; simplify_eq); done.
 Qed.
 
-Lemma head_ctx_step_val p Ki e σ1 e2 σ2 :
+Lemma head_ctx_item_step_val p Ki e σ1 e2 σ2 :
   head_step p (fill_item Ki e) σ1 e2 σ2 → is_Some (to_val e).
 Proof. revert e2. induction Ki. 1-12: inversion_clear 1; simplify_option_eq; eauto.
        - inversion 1. enough (exists k, Val k = e ∧ In k va0) as (k & <- & _) by easy.
@@ -527,16 +553,269 @@ Proof.
     + f_equal. apply (map_inj Val). 2:easy. congruence.
 Qed.
 
-Lemma alloc_fresh p n σ :
-  let l := fresh_locs (dom σ) in
-  (0 < n)%Z →
-  head_step p (Malloc ((Val $ LitV $ LitInt $ n))) σ
-            (Val $ LitV $ LitLoc l) (state_init_heap l n Uninitialized σ).
+Lemma prim_step_inv p e1 e2 σ1 σ2 :
+  prim_step p e1 σ1 e2 σ2 →
+  ∃ K e1' e2', e1 = fill K e1' ∧ e2 = fill K e2' ∧ head_step p e1' σ1 e2' σ2.
+Proof. inversion 1; subst; do 3 eexists; eauto. Qed.
+
+Lemma head_prim_step p e1 σ1 e2 σ2 :
+  head_step p e1 σ1 e2 σ2 → prim_step p e1 σ1 e2 σ2.
+Proof. apply Prim_step with []; by rewrite ?fill_empty. Qed.
+
+Local Lemma fill_val (K : list ectx_item) (e: expr) :
+  is_Some (to_val (fill K e)) → is_Some (to_val e).
+Proof.
+  intros [v Hv]. revert v Hv. induction K as [|k1 K] using rev_ind; intros v Hv.
+  1: done.
+  rewrite fill_app in Hv.
+  destruct k1; cbn in Hv; try congruence.
+Qed.
+
+Local Lemma fill_val_2 (K : list ectx_item) (e: expr) v :
+  fill K e = Val v → is_Some (to_val e).
+Proof. intros HH. eapply (fill_val K). rewrite HH//. Qed.
+
+Lemma to_val_of_call fn vs : to_val (of_call fn vs) = None.
+Proof. rewrite /to_val /of_call //. Qed.
+
+Local Lemma fill_call e K fn vs : fill K e = of_call fn vs → K = [] ∨ is_Some (to_val e).
+Proof.
+  revert e. destruct K as [|k1 K] using rev_ind; intros *; cbn; first by left.
+  rewrite fill_app/=.
+  destruct k1; (try by inversion 1); [|].
+  + destruct (fill K e) eqn:Heq; cbn; (try by inversion 1); [].
+    apply fill_val_2 in Heq; eauto.
+  + destruct vf. destruct l; cbn; (try by inversion 1); []. inversion 1; simplify_eq.
+    clear H.
+  assert (In (fill K e) (map Val vs)) as [vv [Hvv' Hvv]]%in_map_iff.
+  { rewrite -H2; apply in_app_iff; right; now left. }
+  symmetry in Hvv'. apply fill_val_2 in Hvv' as [? ?]. eauto.
+Qed.
+
+Local Lemma fill_comp e K1 K2 :
+  fill K1 (fill K2 e) = fill (comp_ectx K1 K2) e.
+Proof. rewrite /fill /comp_ectx foldl_app//. Qed.
+
+Lemma fill_not_val K e : to_val e = None → to_val (fill K e) = None.
+Proof.
+  intros HH. destruct (to_val (fill K e)) eqn:Heq; try done.
+  destruct (fill_val K e); try done. congruence.
+Qed.
+
+Local Lemma val_prim_step p v σ1 e2 σ2:
+  prim_step p (of_val v) σ1 e2 σ2 → False.
+Proof.
+  inversion 1; subst. symmetry in H0. eapply fill_val_2 in H0 as [? ?].
+  eapply val_head_stuck in H2. congruence.
+Qed.
+
+Lemma head_ctx_step_val' p K e σ1 e2 σ2 :
+  head_step p (fill K e) σ1 e2 σ2 → K = [] ∨ is_Some (to_val e).
+Proof.
+  destruct K as [|Ki K _] using rev_ind; simpl; first by auto.
+  rewrite fill_app /=.
+  intros [v' ?]%head_ctx_item_step_val%fill_val. right. exists v'.
+  by repeat (case_match; simplify_eq).
+Qed.
+
+Lemma head_ctx_step_val p K e σ1 e2 σ2 :
+  head_step p (fill K e) σ1 e2 σ2 → K = [] ∨ is_Some (to_val e).
+Proof.
+  intros [?|[v Hv]]%head_ctx_step_val'; first by left. right.
+  rewrite Hv. eauto.
+Qed.
+
+Lemma step_by_val : ∀ p K' K_redex e1' e1_redex σ1 e2 σ2,
+  fill K' e1' = fill K_redex e1_redex →
+  to_val e1' = None →
+  head_step p e1_redex σ1 e2 σ2 →
+  ∃ K'', K_redex = comp_ectx K' K''.
+Proof.
+  intros p.
+    intros K K' e1 e1' σ1 e2 σ2 Hfill Hred Hstep; revert K' Hfill.
+    induction K as [|Ki K IH] using rev_ind=> /= K' Hfill; eauto using app_nil_r.
+    destruct K' as [|Ki' K' _] using @rev_ind; simplify_eq/=.
+    { rewrite fill_app in Hstep. apply head_ctx_item_step_val in Hstep.
+      apply fill_val in Hstep. destruct Hstep as [? Hstep]. congruence. }
+    rewrite !fill_app /= in Hfill.
+    assert (Ki = Ki') as ->.
+    { eapply fill_item_no_val_inj, Hfill.
+      2: by eapply fill_not_val, val_head_stuck.
+      eapply fill_not_val. by destruct e1. }
+    simplify_eq. destruct (IH K') as [K'' ->]; auto.
+    exists K''. rewrite /comp_ectx assoc //.
+Qed.
+
+Lemma call_head_step (p: gmap string function) f vs σ1 e2 σ2 :
+  head_step p (of_call f vs) σ1 e2 σ2 ↔
+  ∃ (fn : function),
+    p !! f = Some fn ∧ Some e2 = apply_function fn vs ∧ σ2 = σ1.
+Proof.
+  split.
+  - intros H. inversion H; subst. inversion H; subst.
+    repeat econstructor; [apply H2|]. simplify_eq. congruence.
+  - intros ([args ee] & H1 & H2 & ->). econstructor; eauto.
+Qed.
+
+Lemma prim_step_call_inv (p: gmap _ _) K f vs e' σ σ' :
+  prim_step p (fill K (of_call f vs)) σ e' σ' →
+  ∃ er fn, Some er = apply_function fn vs ∧ p !! f = Some fn ∧ e' = fill K er ∧ σ' = σ.
+Proof.
+  intros (K' & e1 & e2 & Hctx & -> & Hstep)%prim_step_inv.
+  eapply step_by_val in Hstep as H'; eauto.
+  destruct H' as [K'' Hctx']; subst K'.
+  rewrite -fill_comp in Hctx. eapply fill_inj in Hctx.
+  destruct (fill_call e1 K'' f vs) as [->|Hval]; auto.
+  - cbn in *; subst. apply call_head_step in Hstep as (?&?&?&?); simplify_eq.
+    do 2 eexists. split_and!; eauto.
+  - eapply val_head_stuck in Hstep. destruct Hval; congruence.
+Qed.
+
+Local Lemma call_prim_step (p: gmap _ _) f vs K e σ1 e' σ2 :
+  is_call e f vs K →
+  prim_step p e σ1 e' σ2 ↔
+  ∃ (fn : function) (e2 : expr),
+    p !! f = Some fn ∧ Some e2 = apply_function fn vs ∧ e' = fill K e2 ∧ σ2 = σ1.
+Proof.
+  unfold is_call. intros Hcall. split.
+  { subst. intros HH%prim_step_call_inv. naive_solver. }
+  { intros (fn & e2 & ? & ? & ? & ?); simplify_eq. econstructor; [done..|].
+    apply call_head_step. eauto. }
+Qed.
+
+Local Lemma is_val_not_call e : is_Some (to_val e) → (∀ f vs C, ¬ is_call e f vs C).
+Proof.
+  destruct e; try by inversion 1. cbn. intros _ *.
+  intros [? ?]%eq_sym%fill_val_2. done.
+Qed.
+
+Local Lemma is_call_in_cont e K1 K2 fn vs :
+  is_call e fn vs K2 →
+  is_call (fill K1 e) fn vs (comp_ectx K1 K2).
+Proof. unfold is_call. rewrite -fill_comp. naive_solver. Qed.
+
+Local Lemma is_call_of_call_inv fn vs fn' vs' K :
+  is_call (of_call fn vs) fn' vs' K →
+  fn' = fn ∧ vs' = vs ∧ K = [].
+Proof.
+  intros *. unfold is_call. intros HH.
+  pose proof (fill_call _ _ _ _ (eq_sym HH)) as [?|?]; subst; cbn in *.
+  * inversion HH; subst. apply stdpp_extra.map_inj in H1; eauto.
+    intros *; by inversion 1.
+  * by inversion H.
+Qed.
+
+Local Lemma prim_step_fill p K e σ e' σ' :
+  prim_step p e σ e' σ' →
+  prim_step p (fill K e) σ (fill K e') σ'.
+Proof.
+  intros (K' & e1' & e2' & -> & -> & ?) % prim_step_inv.
+  rewrite !fill_comp. by econstructor.
+Qed.
+
+Local Lemma fill_step_inv K p e1' σ1 e2 σ2 :
+  to_val e1' = None → prim_step p (fill K e1') σ1 e2 σ2 →
+  ∃ e2', e2 = fill K e2' ∧ prim_step p e1' σ1 e2' σ2.
+Proof.
+  intros H1. inversion 1; simplify_eq.
+  destruct (step_by_val _ _ _ _ _ _ _ _ H0 H1 H3) as (K'' & ->).
+  rewrite <- fill_comp in *.
+  apply fill_inj in H0; simplify_eq. eexists. split; eauto.
+  by econstructor.
+Qed.
+
+Local Lemma head_reducible_prim_step_ctx p K e1 σ1 e2 σ2 :
+  head_reducible p e1 σ1 →
+  prim_step p (fill K e1) σ1 e2 σ2 →
+  ∃ e2', e2 = fill K e2' ∧ head_step p e1 σ1 e2' σ2.
+Proof.
+  intros (e2''&σ2''&HhstepK) (K' & e1' & e2' & HKe1 & -> & Hstep) % prim_step_inv.
+  edestruct (step_by_val p K) as [K'' ?];
+    eauto using val_head_stuck; simplify_eq/=.
+  rewrite -fill_comp in HKe1; simplify_eq.
+  exists (fill K'' e2'). rewrite fill_comp; split; first done.
+  apply head_ctx_step_val in HhstepK as [?|[v ?]]; simplify_eq.
+  - by rewrite //=.
+  - apply val_head_stuck in Hstep; simplify_eq.
+Qed.
+
+Lemma head_reducible_prim_step p e1 σ1 e2 σ2 :
+  head_reducible p e1 σ1 →
+  prim_step p e1 σ1 e2 σ2 →
+  head_step p e1 σ1 e2 σ2.
 Proof.
   intros.
-  apply MallocS; first done.
-  intros. apply not_elem_of_dom.
-  by apply fresh_locs_fresh.
+  edestruct (head_reducible_prim_step_ctx p []) as (?&?&?);
+    rewrite ?fill_empty; eauto.
+  by simplify_eq.
+Qed.
+
+#[local] Notation omap f x := (match x with Some v => f v | None => None end).
+
+Fixpoint unmap_val el :=
+  match el with
+  | Val v :: er => omap (fun vr => Some (v::vr)) (unmap_val er)
+  | [] => Some nil
+  | _ => None
+  end.
+
+Local Definition to_call_head (e : expr) :=
+  match e with
+  | FunCall (Val (LitV (LitFunPtr fn))) el => omap (λ vs, Some (fn, vs)) (unmap_val el)
+  | _ => None
+  end.
+
+Lemma map_unmap_val l : unmap_val (map Val l) = Some l.
+Proof.
+  induction l.
+  - easy.
+  - cbn. rewrite IHl. easy.
+Qed.
+
+Lemma unmap_val_map le lv : unmap_val le = Some lv → map Val lv = le.
+Proof.
+  induction le in lv|-*.
+  - intros H. injection H. intros <-. easy.
+  - cbn. destruct a. 2-12:congruence.
+    destruct (unmap_val le) eqn:Heq. 2:congruence.
+    intros H. injection H. intros <-. cbn. f_equal. now apply IHle.
+Qed.
+
+Local Lemma prim_step_call_dec p e σ e' σ' :
+  prim_step p e σ e' σ' →
+  (∃ fn vs K, is_call e fn vs K) ∨ (∀ fn vs K, ¬ is_call e fn vs K).
+Proof.
+  intros (K & e1' & e2' & ? & ? & Hstep)%prim_step_inv; subst.
+  destruct (to_val e1') eqn:Hval.
+  { exfalso. apply val_head_stuck in Hstep. congruence. }
+
+  destruct (to_call_head e1') as [[fn vs]|] eqn:Hcall.
+  { assert (∃ fn vs, e1' = of_call fn vs) as (fn' & vs' & ?).
+    { unfold to_call_head in Hcall. repeat case_match; simplify_eq.
+      eapply unmap_val_map in H3. subst; eauto. } subst.
+    apply call_head_step in Hstep as (?&?&?&?); simplify_eq.
+    unfold is_call. eauto. }
+
+  right. unfold is_call, of_call.
+  intros fn vs K' Hcall'%eq_sym.
+  pose proof Hcall' as Hcall''.
+  eapply step_by_val in Hcall'' as (?&?); eauto; subst.
+  rewrite -fill_comp in Hcall'. apply fill_inj in Hcall'.
+  symmetry in Hcall'. pose proof Hcall' as Hcall''.
+  apply fill_call in Hcall'' as [|]; cbn in *; subst.
+  - cbn in Hcall'; subst. rewrite /= map_unmap_val // in Hcall.
+  - destruct H; congruence.
+Qed.
+
+Local Lemma prim_step_no_call p1 p2 e σ e' σ' :
+  (∀ f vs K, ¬ is_call e f vs K) →
+  prim_step p1 e σ e' σ' →
+  prim_step p2 e σ e' σ'.
+Proof.
+  intros Hncall (K & e1' & e2' & ? & ? & Hstep)%prim_step_inv; subst.
+  inversion Hstep; subst.
+  all: try repeat (econstructor; eauto).
+  exfalso. eapply Hncall. done.
 Qed.
 
 End C_lang.
