theories/language/language.v
@@ -5,10 +5,12 @@ From melocoton Require Export language_commons.
 
 Section language_mixin.
   Context {expr val func ectx state : Type}.
-  Notation mixin_expr_class := (@mixin_expr_class val).
 
-  Context (of_class : mixin_expr_class → expr).
-  Context (to_class : expr → option mixin_expr_class).
+  Context (of_val : val → expr).
+  Context (to_val : expr → option val).
+
+  Context (of_call : string → list val → expr).
+  Context (is_call : expr → string → list val → ectx → Prop).
 
   Context (empty_ectx : ectx).
   Context (comp_ectx : ectx → ectx → ectx).
@@ -18,64 +20,55 @@ Section language_mixin.
   Local Notation mixin_prog := (gmap string func).
 
   Context (apply_func : func → list val → option expr).
-  Context (head_step : mixin_prog → expr → state → expr → state → Prop).
+  Context (prim_step : mixin_prog → expr → state → expr → state → Prop).
 
   Record LanguageMixin := {
-    (** Expression classification *)
-    mixin_to_of_class c : to_class (of_class c) = Some c;
-    mixin_of_to_class e c : to_class e = Some c → of_class c = e;
+    mixin_to_of_val c : to_val (of_val c) = Some c;
+    mixin_of_to_val e c : to_val e = Some c → of_val c = e;
 
     (** Reduction behavior of the special classes of expressions *)
-    (** mixin_val_head_step is not an iff because the backward direction is trivial *)
-    mixin_val_head_step p v σ1 e2 σ2 :
-      head_step p (of_class (ExprVal v)) σ1 e2 σ2 → False;
-    mixin_call_head_step p f vs σ1 e2 σ2 :
-      head_step p (of_class (ExprCall f vs)) σ1 e2 σ2 ↔
-      ∃ (fn : func),
-        p !! f = Some fn ∧ Some e2 = apply_func fn vs ∧ σ2 = σ1;
-    mixin_call_in_ctx K K' e s' vv :
-      fill K e = fill K' (of_class (ExprCall s' vv))
-      → (∃ K'', K' = comp_ectx K K'') ∨ (∃ v, of_class (ExprVal v) = e);
+    mixin_val_prim_step p v σ1 e2 σ2 :
+      prim_step p (of_val v) σ1 e2 σ2 → False;
+    mixin_call_prim_step p f vs K e σ1 e' σ2 :
+      is_call e f vs K →
+      prim_step p e σ1 e' σ2 ↔
+      ∃ (fn : func) (e2 : expr),
+        p !! f = Some fn ∧ Some e2 = apply_func fn vs ∧ e' = fill K e2 ∧ σ2 = σ1;
 
-    mixin_head_step_mp_call p1 p2 e1 σ1 e2 σ2 :
-      head_step p1 e1 σ1 e2 σ2 → to_class e1 = None → head_step p2 e1 σ1 e2 σ2;
+    (** Same-language linking requires those *)
+    mixin_prim_step_call_dec p e σ e' σ' :
+      prim_step p e σ e' σ' →
+      (∃ fn vs K, is_call e fn vs K) ∨ (∀ fn vs K, ¬ is_call e fn vs K);
+    mixin_prim_step_no_call p1 p2 e σ e' σ' :
+      (∀ f vs K, ¬ is_call e f vs K) →
+      prim_step p1 e σ e' σ' →
+      prim_step p2 e σ e' σ';
 
-    (** Evaluation contexts *)
-    mixin_fill_empty e : fill empty_ectx e = e;
-    mixin_comp_empty_l K: comp_ectx empty_ectx K = K;
-    mixin_comp_empty_r K : comp_ectx K empty_ectx = K;
-    mixin_fill_comp K1 K2 e : fill K1 (fill K2 e) = fill (comp_ectx K1 K2) e;
-    mixin_fill_inj K : Inj (=) (=) (fill K);
-    (* The the things in a class contain only values in redex positions (or the
-       redex is the topmost one). *)
-    mixin_fill_class K e :
-      is_Some (to_class (fill K e)) → K = empty_ectx ∨ ∃ v, to_class e = Some (ExprVal v);
+    mixin_is_val_not_call e : is_Some (to_val e) → (∀ f vs K, ¬ is_call e f vs K);
+    mixin_is_call_in_cont e K1 K2 fn vs :
+      is_call e fn vs K2 → is_call (fill K1 e) fn vs (comp_ectx K1 K2);
+    mixin_of_call_is_call fn vs : is_call (of_call fn vs) fn vs empty_ectx;
+    mixin_is_call_of_call e fn vs K : is_call e fn vs K → e = fill K (of_call fn vs);
+    mixin_is_call_of_call_inv fn vs fn' vs' K :
+      is_call (of_call fn vs) fn' vs' K →
+      fn' = fn ∧ vs' = vs ∧ K = empty_ectx;
 
-    (** Given a head redex [e1_redex] somewhere in a term, and another
-        decomposition of the same term into [fill K' e1'] such that [e1'] is not
-        a value, then the head redex context is [e1']'s context [K'] filled with
-        another context [K''].  In particular, this implies [e1 = fill K''
-        e1_redex] by [fill_inj], i.e., [e1]' contains the head redex.)
+    mixin_fill_val e K : is_Some (to_val (fill K e)) → is_Some (to_val e);
+    mixin_fill_comp e K1 K2 :
+      fill K1 (fill K2 e) = fill (comp_ectx K1 K2) e;
+    mixin_fill_empty e :
+      fill empty_ectx e = e;
 
-        This implies there can be only one head redex, see
-        [head_redex_unique]. *)
-    mixin_step_by_val p K' K_redex e1' e1_redex σ1 e2 σ2 :
-      fill K' e1' = fill K_redex e1_redex →
-      match to_class e1' with Some (ExprVal _) => False | _ => True end →
-      head_step p e1_redex σ1 e2 σ2 →
-      ∃ K'', K_redex = comp_ectx K' K'';
-
-    (** If [fill K e] takes a head step, then either [e] is a value or [K] is
-        the empty evaluation context. In other words, if [e] is not a value
-        wrapping it in a context does not add new head redex positions. *)
-    (* FIXME: This is the exact same conclusion as [mixin_fill_class]... is
-       there some pattern or reduncancy here? *)
-    mixin_head_ctx_step_val p K e σ1 e2 σ2 :
-      head_step p (fill K e) σ1 e2 σ2 → K = empty_ectx ∨ ∃ v, to_class e = Some (ExprVal v);
+    (** Those are key for proving [wp_bind] *)
+    mixin_prim_step_fill p K e σ e' σ' :
+      prim_step p e σ e' σ' →
+      prim_step p (fill K e) σ (fill K e') σ';
+    mixin_fill_step_inv p K e1' σ1 e2 σ2 :
+      to_val e1' = None → prim_step p (fill K e1') σ1 e2 σ2 →
+      ∃ e2', e2 = fill K e2' ∧ prim_step p e1' σ1 e2' σ2;
   }.
 End language_mixin.
 
-Arguments mixin_expr_class : clear implicits.
 Global Notation mixin_prog func := (gmap string func).
 
 Structure language {val : Type} := Language {
@@ -84,49 +77,39 @@ Structure language {val : Type} := Language {
   ectx : Type;
   state : Type;
 
-  of_class : mixin_expr_class val → expr;
-  to_class : expr → option (mixin_expr_class val);
+  of_val : val → expr;
+  to_val : expr → option val;
+  of_call : string → list val → expr;
+  is_call : expr → string → list val → ectx → Prop;
+
   empty_ectx : ectx;
   comp_ectx : ectx → ectx → ectx;
   fill : ectx → expr → expr;
   apply_func : func → list val → option expr;
-  head_step : mixin_prog func → expr → state → expr → state → Prop;
+  prim_step : mixin_prog func → expr → state → expr → state → Prop;
 
   language_mixin :
-    LanguageMixin (val:=val) of_class to_class empty_ectx comp_ectx fill
-      apply_func head_step
+    LanguageMixin of_val to_val of_call is_call  empty_ectx comp_ectx fill
+      apply_func prim_step
 }.
 
 Declare Scope expr_scope.
 Bind Scope expr_scope with expr.
 
 Arguments language : clear implicits.
-Arguments Language {_ expr _ _ _ _ _ _ _ _ apply_func head_step}.
-Arguments of_class {_} _ _.
-Arguments to_class {_ _} _.
+Arguments Language {_ expr _ _ _ _ _ _ _ _ _ _ apply_func prim_step}.
+Arguments of_val {_} _ _.
+Arguments to_val {_ _} _.
+Arguments of_call {_} _ _.
+Arguments is_call {_ _}.
 Arguments empty_ectx {_ _}.
 Arguments comp_ectx {_ _} _ _.
 Arguments fill {_ _} _ _.
 Arguments apply_func {_ _}.
-Arguments head_step {_ _} _ _ _ _ _.
+Arguments prim_step {_ _} _ _ _ _ _.
 
-Definition expr_class {val} (Λ : language val) := mixin_expr_class val.
 (* A [Definition] throws off Coq's "old" ("tactic") unification engine *)
 Notation prog Λ := (mixin_prog Λ.(func)).
-
-Definition to_val {val} {Λ : language val} (e : expr Λ) :=
-  match to_class e with
-  | Some (ExprVal v) => Some v
-  | _ => None
-  end.
-Definition of_val {val} (Λ : language val) (v : val) := of_class Λ (ExprVal v).
-
-Definition to_call {val} {Λ : language val} (e : expr Λ) :=
-  match to_class e with
-  | Some (ExprCall f v) => Some (f, v)
-  | _ => None
-  end.
-Definition of_call {val} (Λ : language val) f (v : list val) := of_class Λ (ExprCall f v).
 
 (* From an ectx_language, we can construct a language. *)
 Section language.
@@ -135,435 +118,118 @@ Section language.
   Implicit Types v : val.
   Implicit Types vs : list val.
   Implicit Types e : expr Λ.
-  Implicit Types c : expr_class Λ.
   Implicit Types K : ectx Λ.
   Implicit Types p : prog Λ.
 
-  Lemma to_of_class c : to_class (of_class Λ c) = Some c.
+  Lemma to_of_val v : to_val (of_val Λ v) = Some v.
   Proof. apply language_mixin. Qed.
-  Lemma of_to_class e c : to_class e = Some c → of_class Λ c = e.
+  Lemma of_to_val e v : to_val e = Some v → of_val Λ v = e.
   Proof. apply language_mixin. Qed.
 
-  Lemma of_class_inj k1 k2 : of_class Λ k1 = of_class Λ k2 -> k1 = k2.
+  Lemma of_val_inj v1 v2 : of_val Λ v1 = of_val Λ v2 → v1 = v2.
   Proof.
-    intros H. enough (Some k1 = Some k2) by congruence.
-    rewrite <- !to_of_class. rewrite H. done.
+    intros H. enough (Some v1 = Some v2) by congruence.
+    rewrite <- !to_of_val. rewrite H. done.
   Qed.
 
-  Lemma to_val_of_call f vs : to_val (of_call Λ f vs) = None.
-  Proof. rewrite /to_val /of_call to_of_class. done. Qed.
-  Lemma to_call_of_val v : to_call (of_val Λ v) = None.
-  Proof. rewrite /to_call /of_val to_of_class. done. Qed.
-  Lemma is_val_is_class e : is_Some (to_val e) → is_Some (to_class e).
-  Proof. rewrite /to_val /is_Some. destruct (to_class e) as [[|]|]; naive_solver. Qed.
-  Lemma is_call_is_class e : is_Some (to_call e) → is_Some (to_class e).
-  Proof. rewrite /to_call /is_Some. destruct (to_class e) as [[|]|]; naive_solver. Qed.
+  Lemma val_prim_step p v σ1 e2 σ2 :
+    prim_step p (of_val Λ v) σ1 e2 σ2 → False.
+  Proof. apply language_mixin. Qed.
+  Lemma call_prim_step p fn vs K e σ1 e' σ2 :
+    is_call e fn vs K →
+    prim_step p e σ1 e' σ2 ↔
+    ∃ (f : func Λ) e2, p !! fn = Some f ∧ Some e2 = apply_func f vs ∧ e' = fill K e2 ∧ σ2 = σ1.
+  Proof. apply language_mixin. Qed.
+  Lemma prim_step_call_dec p e σ e' σ' :
+    prim_step p e σ e' σ' →
+    (∃ fn vs K, is_call e fn vs K) ∨ (∀ fn vs K, ¬ is_call e fn vs K).
+  Proof. apply language_mixin. Qed.
+  Lemma prim_step_no_call p1 p2 e σ e' σ' :
+    (∀ f vs K, ¬ is_call e f vs K) →
+    prim_step p1 e σ e' σ' →
+    prim_step p2 e σ e' σ'.
+  Proof. apply language_mixin. Qed.
 
-  Lemma val_head_step p v σ1 e2 σ2 :
-    head_step p (of_class Λ (ExprVal v)) σ1 e2 σ2 → False.
+  Lemma is_val_not_call e : is_Some (to_val e) → (∀ f vs C, ¬ is_call e f vs C).
   Proof. apply language_mixin. Qed.
-  Lemma call_head_step p f vs σ1 e2 σ2 :
-    head_step p (of_class Λ (ExprCall f vs)) σ1 e2 σ2 ↔
-    ∃ fn, p !! f = Some fn ∧ Some e2 = apply_func fn vs ∧ σ2 = σ1.
-  Proof. apply language_mixin. Qed.
-
-  Lemma fill_empty e : fill empty_ectx e = e.
-  Proof. apply language_mixin. Qed.
-  Lemma comp_empty_l K: comp_ectx empty_ectx K = K.
-  Proof. apply language_mixin. Qed.
-  Lemma comp_empty_r K : comp_ectx K empty_ectx = K.
-  Proof. apply language_mixin. Qed.
-  Lemma fill_comp K1 K2 e : fill K1 (fill K2 e) = fill (comp_ectx K1 K2) e.
-  Proof. apply language_mixin. Qed.
-  Global Instance fill_inj K : Inj (=) (=) (fill K).
-  Proof. apply language_mixin. Qed.
-  Lemma fill_class' K e :
-    is_Some (to_class (fill K e)) → K = empty_ectx ∨ ∃ v, to_class e = Some (ExprVal v).
-  Proof. apply language_mixin. Qed.
-  Lemma step_by_val' p K' K_redex e1' e1_redex σ1 e2 σ2 :
-      fill K' e1' = fill K_redex e1_redex →
-      match to_class e1' with Some (ExprVal _) => False | _ => True end →
-      head_step p e1_redex σ1 e2 σ2 →
-      ∃ K'', K_redex = comp_ectx K' K''.
-  Proof. apply language_mixin. Qed.
-  Lemma head_ctx_step_val' p K e σ1 e2 σ2 :
-    head_step p (fill K e) σ1 e2 σ2 → K = empty_ectx ∨ ∃ v, to_class e = Some (ExprVal v).
-  Proof. apply language_mixin. Qed.
-  Lemma call_in_ctx K K' e s' vv : 
-      fill K e = fill K' (of_class _ (ExprCall s' vv))
-      → (∃ K'', K' = comp_ectx K K'') ∨ (∃ v, of_class _ (ExprVal v) = e).
-  Proof. apply language_mixin. Qed.
-  Lemma call_in_ctx_to_val K K' e s' vv : 
-      fill K e = fill K' (of_class _ (ExprCall s' vv))
-      → (∃ K'', K' = comp_ectx K K'') ∨ is_Some (to_val e).
+  Lemma is_val_not_call_2 e f vs C : is_call e f vs C → to_val e = None.
   Proof.
-    intros [H1|(x&Hx)]%call_in_ctx.
-    - by left.
-    - right. exists x. unfold to_val. rewrite <- Hx. now rewrite to_of_class.
-  Qed.
-  Lemma fill_class K e :
-    is_Some (to_class (fill K e)) → K = empty_ectx ∨ is_Some (to_val e).
-  Proof.
-    intros [?|[v Hv]]%fill_class'; first by left. right.
-    rewrite /to_val Hv. eauto.
-  Qed.
-  Lemma to_val_fill_call K f vs :
-    to_val (fill K (of_call Λ f vs)) = None.
-  Proof.
-    destruct (to_val (fill K (of_call Λ f vs))) eqn:HH; eauto.
-    destruct (fill_class K (of_call Λ f vs)) as [H1|H2].
-    { unfold to_val in HH. repeat case_match; simplify_eq. eauto. }
-    { subst. rewrite fill_empty in HH. unfold to_val in HH.
-      repeat case_match; simplify_eq.
-      unfold of_call in *. by rewrite -> to_of_class in *. }
-    { clear HH. rewrite -> to_val_of_call in H2. by apply is_Some_None in H2. }
-  Qed.
-  Lemma call_call_in_ctx K K' fn fn' vs vs' :
-    fill K (of_class _ (ExprCall fn vs)) = fill K' (of_class _ (ExprCall fn' vs')) →
-    K' = K ∧ fn' = fn ∧ vs' = vs.
-  Proof.
-    intros HH. destruct (call_in_ctx _ _ _ _ _ HH) as [[K'' ->]|[? H2]].
-    { rewrite -fill_comp in HH. apply fill_inj in HH.
-      destruct (fill_class K'' (of_class _ (ExprCall fn' vs'))) as [Hc|Hc].
-      { rewrite -HH /= to_of_class //. }
-      2: { exfalso. rewrite /to_val to_of_class in Hc. by apply is_Some_None in Hc. }
-      subst K''. rewrite fill_empty in HH. rewrite comp_empty_r. apply of_class_inj in HH. by simplify_eq. }
-    { exfalso. apply of_class_inj in H2. congruence. }
+    intros H; destruct (to_val e) eqn:Heq; try done.
+    exfalso; apply mk_is_Some in Heq.
+    eapply is_val_not_call in Heq. done.
   Qed.
 
-  Lemma head_step_no_call p1 p2 e1 σ1 e2 σ2 :
-      head_step p1 e1 σ1 e2 σ2 → to_class e1 = None → head_step p2 e1 σ1 e2 σ2.
+  Lemma is_call_in_cont e K1 K2 fn vs :
+    is_call e fn vs K2 → is_call (fill K1 e) fn vs (comp_ectx K1 K2).
+  Proof. apply language_mixin. Qed.
+
+  Lemma of_call_is_call fn vs : is_call (of_call Λ fn vs) fn vs empty_ectx.
+  Proof. apply language_mixin. Qed.
+  Lemma is_call_of_call e fn vs K : is_call e fn vs K → e = fill K (of_call Λ fn vs).
+  Proof. apply language_mixin. Qed.
+  Lemma is_call_of_call_inv fn vs fn' vs' K :
+    is_call (of_call Λ fn vs) fn' vs' K →
+    fn' = fn ∧ vs' = vs ∧ K = empty_ectx.
+  Proof. apply language_mixin. Qed.
+
+  Lemma fill_val e K : is_Some (to_val (fill K e)) → is_Some (to_val e).
+  Proof. apply language_mixin. Qed.
+  Lemma fill_val_2 K e v : fill K e = of_val Λ v → is_Some (to_val e).
+  Proof. intros HH. eapply (fill_val _ K). rewrite HH to_of_val//. Qed.
+
+  Lemma fill_not_val e K : to_val e = None → to_val (fill K e) = None.
   Proof.
-    apply language_mixin.
+    intros Heq; destruct (to_val (fill K e)) as [v|] eqn:Heq2; last done.
+    eapply mk_is_Some in Heq2. apply fill_val in Heq2. rewrite Heq in Heq2.
+    by destruct Heq2.
   Qed.
 
-  Lemma step_by_val p K' K_redex e1' e1_redex σ1 e2 σ2 :
-      fill K' e1' = fill K_redex e1_redex →
-      to_val e1' = None →
-      head_step p e1_redex σ1 e2 σ2 →
-      ∃ K'', K_redex = comp_ectx K' K''.
+  Lemma fill_comp e K1 K2 :
+    fill K1 (fill K2 e) = fill (comp_ectx K1 K2) e.
+  Proof. apply language_mixin. Qed.
+  Lemma fill_empty e :
+    fill empty_ectx e = e.
+  Proof. apply language_mixin. Qed.
+
+  Lemma val_stuck p e σ e' σ' : prim_step p e σ e' σ' → to_val e = None.
   Proof.
-    rewrite /to_val => ? He1'. eapply step_by_val'; first done.
-    destruct (to_class e1') as [[]|]; done.
+    intros Hstep. destruct (to_val e) eqn:HH; eauto. apply of_to_val in HH; subst.
+    by apply val_prim_step in Hstep.
   Qed.
-  Lemma head_ctx_step_val p K e σ1 e2 σ2 :
-    head_step p (fill K e) σ1 e2 σ2 → K = empty_ectx ∨ is_Some (to_val e).
-  Proof.
-    intros [?|[v Hv]]%head_ctx_step_val'; first by left. right.
-    rewrite /to_val Hv. eauto.
-  Qed.
-  Lemma call_head_step_inv p f vs σ1 e2 σ2 :
-    head_step p (of_class Λ (ExprCall f vs)) σ1 e2 σ2 →
-    ∃ fn, p !! f = Some fn ∧ Some e2 = apply_func fn vs ∧ σ2 = σ1.
-  Proof. eapply call_head_step. Qed.
-  Lemma call_head_step_intro p f vs fn σ1 er :
-    p !! f = Some fn →
-    Some er = apply_func fn vs →
-    head_step p (of_call Λ f vs) σ1 er σ1.
-  Proof. intros ? ?. eapply call_head_step; eexists; eauto. Qed.
 
-  Definition head_reducible (p : prog Λ) (e : expr Λ) (σ : state Λ) :=
-    ∃ e' σ', head_step p e σ e' σ'.
-  Definition head_irreducible (p : prog Λ) (e : expr Λ) (σ : state Λ) :=
-    ∀ e' σ', ¬head_step p e σ e' σ'.
-  Definition head_stuck (p : prog Λ) (e : expr Λ) (σ : state Λ) :=
-    to_val e = None ∧ head_irreducible p e σ.
-
-  (* All non-value redexes are at the root.  In other words, all sub-redexes are
-     values. *)
-  Definition sub_redexes_are_values (e : expr Λ) :=
-    ∀ K e', e = fill K e' → to_val e' = None → K = empty_ectx.
-
-  Inductive prim_step (p : prog Λ) : expr Λ → state Λ → expr Λ → state Λ → Prop :=
-    Prim_step K e1 e2 σ1 σ2 e1' e2' :
-      e1 = fill K e1' → e2 = fill K e2' →
-      head_step p e1' σ1 e2' σ2 → prim_step p e1 σ1 e2 σ2.
-
-  Lemma Prim_step' p K e1 σ1 e2 σ2 :
-    head_step p e1 σ1 e2 σ2 → prim_step p (fill K e1) σ1 (fill K e2) σ2.
-  Proof. econstructor; eauto. Qed.
+  Lemma prim_step_fill p K e σ e' σ' :
+    prim_step p e σ e' σ' →
+    prim_step p (fill K e) σ (fill K e') σ'.
+  Proof. apply language_mixin. Qed.
 
   Definition reducible (p : prog Λ) (e : expr Λ) (σ : state Λ) :=
     ∃ e' σ', prim_step p e σ e' σ'.
-  Definition irreducible (p : prog Λ) (e : expr Λ) (σ : state Λ) :=
-    ∀ e' σ', ¬prim_step p e σ e' σ'.
-  Definition stuck (p : prog Λ) (e : expr Λ) (σ : state Λ) :=
-    to_val e = None ∧ irreducible p e σ.
-  Definition not_stuck (p : prog Λ) (e : expr Λ) (σ : state Λ) :=
-    is_Some (to_val e) ∨ reducible p e σ.
 
-  (** Some lemmas about this language *)
-  Lemma prim_step_inv p e1 e2 σ1 σ2 :
-    prim_step p e1 σ1 e2 σ2 →
-    ∃ K e1' e2', e1 = fill K e1' ∧ e2 = fill K e2' ∧ head_step p e1' σ1 e2' σ2.
-  Proof. inversion 1; subst; do 3 eexists; eauto. Qed.
-  Lemma to_of_val v : to_val (of_val Λ v) = Some v.
-  Proof. rewrite /to_val /of_val to_of_class //. Qed.
-  Lemma of_to_val e v : to_val e = Some v → of_val Λ v = e.
-  Proof.
-    rewrite /to_val /of_val => Hval. apply of_to_class.
-    destruct (to_class e) as [[]|]; simplify_option_eq; done.
-  Qed.
-  Lemma of_to_val_flip v e : of_val Λ v = e → to_val e = Some v.
-  Proof. intros <-. by rewrite to_of_val. Qed.
-  Lemma val_head_stuck p e σ e' σ' : head_step p e σ e' σ' → to_val e = None.
-  Proof.
-    destruct (to_val e) as [v|] eqn:Hval; last done.
-    rewrite -(of_to_val e v) //. intros []%val_head_step.
-  Qed.
-  Lemma fill_val K e : is_Some (to_val (fill K e)) → is_Some (to_val e).
-  Proof.
-    intros Hval. destruct (fill_class K e) as [HK|He].
-    - apply is_val_is_class. done.
-    - subst K. move: Hval. rewrite fill_empty. done.
-    - done.
-  Qed.
-  Lemma val_stuck p e σ e' σ' : prim_step p e σ e' σ' → to_val e = None.
-  Proof.
-    intros (?&?&? & -> & -> & ?%val_head_stuck)%prim_step_inv.
-    apply eq_None_not_Some. by intros ?%fill_val%eq_None_not_Some.
-  Qed.
-
-  Lemma to_of_call f vs : to_call (of_call Λ f vs) = Some (f, vs).
-  Proof. rewrite /to_call /of_call to_of_class //. Qed.
-  Lemma of_to_call e f vs : to_call e = Some (f, vs) → of_call Λ f vs = e.
-  Proof.
-    rewrite /to_call /of_call => Hval. apply of_to_class.
-    destruct (to_class e) as [[] | ]; simplify_option_eq; done.
-  Qed.
-  Lemma of_to_call_flip f vs e : of_call Λ f vs = e → to_call e = Some (f, vs).
-  Proof. intros <-. apply to_of_call. Qed.
-
-  Lemma not_reducible p e σ : ¬reducible p e σ ↔ irreducible p e σ.
-  Proof. unfold reducible, irreducible. naive_solver. Qed.
   Lemma reducible_not_val p e σ : reducible p e σ → to_val e = None.
   Proof. intros (?&?&?); eauto using val_stuck. Qed.
-  Lemma val_irreducible p e σ : is_Some (to_val e) → irreducible p e σ.
-  Proof. intros [??] ?? ?%val_stuck. by destruct (to_val e). Qed.
-  Global Instance of_val_inj : Inj (=) (=) (@of_val _ Λ). 
-  Proof. by intros v v' Hv; apply (inj Some); rewrite -!to_of_val Hv. Qed.
-  Lemma not_not_stuck p e σ : ¬not_stuck p e σ ↔ stuck p e σ.
-  Proof.
-    rewrite /stuck /not_stuck -not_eq_None_Some -not_reducible.
-    destruct (decide (to_val e = None)); naive_solver.
-  Qed.
-
-  Lemma fill_not_val K e : to_val e = None → to_val (fill K e) = None.
-  Proof. rewrite !eq_None_not_Some. eauto using fill_val. Qed.
-
-  Lemma not_head_reducible p e σ : ¬head_reducible p e σ ↔ head_irreducible p e σ.
-  Proof. unfold head_reducible, head_irreducible. naive_solver. Qed.
-
-  (** The decomposition into head redex and context is unique.
-
-      In all sensible instances, [comp_ectx K' empty_ectx] will be the same as
-      [K'], so the conclusion is [K = K' ∧ e = e'], but we do not require a law
-      to actually prove that so we cannot use that fact here. *)
-  Lemma head_redex_unique p K K' e e' σ :
-    fill K e = fill K' e' →
-    head_reducible p e σ →
-    head_reducible p e' σ →
-    K = comp_ectx K' empty_ectx ∧ e = e'.
-  Proof.
-    intros Heq (e2 & σ2 & Hred) (e2' & σ2' & Hred').
-    edestruct (step_by_val p K' K e' e) as [K'' HK];
-      [by eauto using val_head_stuck..|].
-    subst K. move: Heq. rewrite -fill_comp. intros <-%(inj (fill _)).
-    destruct (head_ctx_step_val _ _ _ _ _ _ Hred') as [HK''|[]%not_eq_None_Some].
-    - subst K''. rewrite fill_empty. done.
-    - by eapply val_head_stuck.
-  Qed.
-
-  Lemma head_prim_step p e1 σ1 e2 σ2 :
-    head_step p e1 σ1 e2 σ2 → prim_step p e1 σ1 e2 σ2.
-  Proof. apply Prim_step with empty_ectx; by rewrite ?fill_empty. Qed.
-
-  Lemma head_step_not_stuck p e σ e' σ' :
-    head_step p e σ e' σ' → not_stuck p e σ.
-  Proof. rewrite /not_stuck /reducible /=. eauto 10 using head_prim_step. Qed.
-
-  Lemma fill_prim_step p K e1 σ1 e2 σ2 :
-    prim_step p e1 σ1 e2 σ2 → prim_step p (fill K e1) σ1 (fill K e2) σ2.
-  Proof.
-    intros (K' & e1' & e2' & -> & -> & ?) % prim_step_inv.
-    rewrite !fill_comp. by econstructor.
-  Qed.
-  Lemma fill_reducible p K e σ : reducible p e σ → reducible p (fill K e) σ.
-  Proof.
-    intros (e'&σ'&?). exists (fill K e'), σ'. by apply fill_prim_step.
-  Qed.
-  Lemma head_prim_reducible p e σ : head_reducible p e σ → reducible p e σ.
-  Proof. intros (e'&σ'&?). eexists e', σ'. by apply head_prim_step. Qed.
-  Lemma head_prim_fill_reducible p e K σ :
-    head_reducible p e σ → reducible p (fill K e) σ.
-  Proof. intro. by apply fill_reducible, head_prim_reducible. Qed.
-  Lemma head_prim_irreducible p e σ : irreducible p e σ → head_irreducible p e σ.
-  Proof.
-    rewrite -not_reducible -not_head_reducible. eauto using head_prim_reducible.
-  Qed.
-
-  Lemma prim_head_step p e σ e' σ' :
-    prim_step p e σ e' σ' → sub_redexes_are_values e → head_step p e σ e' σ'.
-  Proof.
-    intros Hprim ?. destruct (prim_step_inv _ _ _ _ _ Hprim) as (K & e1' & e2' & -> & -> & Hstep).
-    assert (K = empty_ectx) as -> by eauto 10 using val_head_stuck.
-    rewrite !fill_empty /head_reducible; eauto.
-  Qed.
-  Lemma prim_head_reducible p e σ :
-    reducible p e σ → sub_redexes_are_values e → head_reducible p e σ.
-  Proof. intros (e'&σ'&Hprim) ?. do 2 eexists; by eapply prim_head_step. Qed.
-  Lemma prim_head_irreducible p e σ :
-    head_irreducible p e σ → sub_redexes_are_values e → irreducible p e σ.
-  Proof.
-    rewrite -not_reducible -not_head_reducible. eauto using prim_head_reducible.
-  Qed.
-
-  Lemma head_stuck_stuck p e σ :
-    head_stuck p e σ → sub_redexes_are_values e → stuck p e σ.
-  Proof.
-    intros [] ?. split; first done. by apply prim_head_irreducible.
-  Qed.
-
-  Lemma head_reducible_prim_step_ctx p K e1 σ1 e2 σ2 :
-    head_reducible p e1 σ1 →
-    prim_step p (fill K e1) σ1 e2 σ2 →
-    ∃ e2', e2 = fill K e2' ∧ head_step p e1 σ1 e2' σ2.
-  Proof.
-    intros (e2''&σ2''&HhstepK) (K' & e1' & e2' & HKe1 & -> & Hstep) % prim_step_inv.
-    edestruct (step_by_val p K) as [K'' ?];
-      eauto using val_head_stuck; simplify_eq/=.
-    rewrite -fill_comp in HKe1; simplify_eq.
-    exists (fill K'' e2'). rewrite fill_comp; split; first done.
-    apply head_ctx_step_val in HhstepK as [?|[v ?]]; simplify_eq.
-    - by rewrite !fill_empty.
-    - apply val_head_stuck in Hstep; simplify_eq.
-  Qed.
-
-  Lemma head_reducible_prim_step p e1 σ1 e2 σ2 :
-    head_reducible p e1 σ1 →
-    prim_step p e1 σ1 e2 σ2 →
-    head_step p e1 σ1 e2 σ2.
-  Proof.
-    intros.
-    edestruct (head_reducible_prim_step_ctx p empty_ectx) as (?&?&?);
-      rewrite ?fill_empty; eauto.
-    by simplify_eq; rewrite fill_empty.
-  Qed.
-
-
-  Lemma reducible_mono p1 p2 e σ : p1 ⊆ p2 → reducible p1 e σ → reducible p2 e σ.
-  Proof.
-    intros Hsub (e2 & σ2 & (K & e1' & e2' & -> & -> & H)%prim_step_inv).
-    exists (fill K e2'), σ2. econstructor; first done. 1:done.
-    destruct (to_class e1') as [[]|] eqn:Heq.
-    - exfalso. eapply val_head_step. apply of_to_class in Heq. erewrite Heq. done.
-    - apply of_to_class in Heq. subst e1'. apply call_head_step in H.
-      destruct H as (Fn & HFn & Happly & ->).
-      apply call_head_step. exists Fn. repeat split; try done.
-      eapply lookup_weaken; done. 
-    - eapply head_step_no_call; done. 
-  Qed.
-
-  Lemma fill_stuck (P : prog Λ) e σ K : stuck P e σ → stuck P (fill K e) σ.
-  Proof.
-    intros Hstuck; split.
-    + apply fill_not_val, Hstuck.
-    + intros e'' σ'' (K_redex &e1 &e2 &Heq &-> &Hhead)%prim_step_inv.
-      edestruct (step_by_val P K K_redex _ _ _ _ _ Heq ltac:(apply Hstuck) Hhead) as (K'' & ->).
-      rewrite -fill_comp in Heq. apply fill_inj in Heq as ->.
-      eapply (proj2 Hstuck). econstructor; eauto.
-  Qed.
-
-  Lemma fill_not_stuck (P : prog Λ) e σ K : not_stuck P (fill K e) σ → not_stuck P e σ.
-  Proof.
-    intros [Hval | Hred].
-    - left. by eapply fill_val.
-    - destruct Hred as (e' & σ' & (K_redex &e1 &e2 &Heq &-> &Hhead)%prim_step_inv).
-      destruct (decide (to_val e = None)) as [Hnval | Hval]; first last.
-      { left. destruct (to_val e) as [v | ]; by eauto. }
-      edestruct (step_by_val P K K_redex _ _ _ _ _ Heq Hnval Hhead) as (K'' & ->).
-      rewrite -fill_comp in Heq. apply fill_inj in Heq as ->.
-      right. eexists _, _. econstructor; eauto.
-  Qed.
-
-  Lemma prim_step_call_inv p K f vs e' σ σ' :
-    prim_step p (fill K (of_call Λ f vs)) σ e' σ' →
-    ∃ er fn, Some er = apply_func fn vs ∧ p !! f = Some fn ∧ e' = fill K er ∧ σ' = σ.
-  Proof.
-    intros (K' & e1 & e2 & Hctx & -> & Hstep)%prim_step_inv.
-    eapply step_by_val in Hstep as H'; eauto; last apply to_val_of_call.
-    destruct H' as [K'' Hctx']; subst K'.
-    rewrite -fill_comp in Hctx. eapply fill_inj in Hctx.
-    destruct (fill_class K'' e1) as [->|Hval].
-    - apply is_call_is_class. erewrite of_to_call_flip; eauto.
-    - rewrite fill_empty in Hctx. subst e1. exists e2.
-      apply call_head_step_inv in Hstep as (fn & ? & -> & ->).
-      exists fn. rewrite -fill_comp fill_empty. naive_solver.
-    - unfold is_Some in Hval. erewrite val_head_stuck in Hval; naive_solver.
-  Qed.
-
-  Lemma val_prim_step p v σ e' σ' :
-   ¬ prim_step p (of_val Λ v) σ e' σ'.
-  Proof.
-    intros (K & e1' & e2' & Heq & -> & Hstep') % prim_step_inv.
-    edestruct (fill_val K e1') as (v1''& ?).
-    { rewrite -Heq. rewrite to_of_val. by exists v. }
-    eapply val_head_step.
-    erewrite <-(of_to_val e1') in Hstep'; eauto.
-  Qed.
-
-  Lemma fill_reducible_prim_step p e e' σ σ' K :
-    reducible p e σ → prim_step p (fill K e) σ e' σ' → ∃ e'', e' = fill K e'' ∧ prim_step p e σ e'' σ'.
-  Proof.
-    intros (e1 & σ1 & (K'' & e1'' & e2'' & ->  & -> & Hhead) % prim_step_inv) Hprim.
-    rewrite fill_comp in Hprim.
-    eapply head_reducible_prim_step_ctx in Hprim as (e1' & -> & Hhead'); last by rewrite /head_reducible; eauto.
-    eexists. rewrite -fill_comp; by eauto using Prim_step'.
-  Qed.
 
   Lemma reducible_fill p e σ K : reducible p e σ → reducible p (fill K e) σ.
   Proof.
-    intros (e' & σ' & Hs). inversion Hs; subst.
-    eexists (fill (comp_ectx K K0) e2'), σ'.
-    econstructor; rewrite ?fill_comp //.
+    intros HH. pose proof (reducible_not_val _ _ _ HH).
+    destruct HH as (e' & σ' & Hs).
+    eexists (fill K e'), σ'. eapply prim_step_fill; eauto.
   Qed.
 
-  Lemma reducible_call_is_in_prog p e K σ s vv :
-    reducible p (fill K e) σ →
-    to_call e = Some (s,vv) →
-    p !! s <> None.
+  Lemma reducible_mono p1 p2 e σ : p1 ⊆ p2 → reducible p1 e σ → reducible p2 e σ.
   Proof.
-    intros [e' [σ' Hred]] H2. unfold to_call in H2. destruct to_class as [[]|] eqn:Heq; try congruence.
-    apply of_to_class in Heq as Heq2; subst. injection H2; intros -> ->.
-    apply prim_step_call_inv in Hred.
-    destruct Hred as (er & fn & Her & Hfn & _).
-    rewrite Hfn; congruence.
+    intros Hsub (?&?&Hstep).
+    pose proof Hstep as Hstep'. apply prim_step_call_dec in Hstep'.
+    destruct Hstep' as [(?&?&?&Hcall)|Hncall].
+    { eapply call_prim_step in Hstep; last done. destruct Hstep as (?&?&?&?&?&?); simplify_eq.
+      eexists _, _. eapply call_prim_step; eauto. eexists _, _. split_and!; eauto.
+      eapply lookup_weaken; eauto. }
+    { eapply prim_step_no_call in Hstep; eauto. by eexists _, _. }
   Qed.
 
   Lemma fill_step_inv K p e1' σ1 e2 σ2 :
     to_val e1' = None → prim_step p (fill K e1') σ1 e2 σ2 →
     ∃ e2', e2 = fill K e2' ∧ prim_step p e1' σ1 e2' σ2.
-  Proof.
-    intros H1. inversion 1; simplify_eq.
-    destruct (step_by_val _ _ _ _ _ _ _ _ H0 H1 H3) as (K'' & ->).
-    rewrite <- fill_comp in *.
-    apply fill_inj in H0; simplify_eq. eexists. split; eauto.
-    by econstructor.
-  Qed.
-
-  Lemma fill_inv p K e σ : to_val e = None → reducible p (fill K e) σ → reducible p e σ.
-  Proof.
-    intros H1 (e'&σ'&(e2'&->&H2)%fill_step_inv). 2:easy.
-    exists e2',σ'. easy.
-  Qed.
-
-  Lemma head_call_pure p f vs σ e2 σ' σ2 :
-    head_step p (of_class Λ (ExprCall f vs)) σ e2 σ' →
-    head_step p (of_class Λ (ExprCall f vs)) σ2 e2 σ2.
-  Proof.
-    intros (fn & H1 & H2 & H3)%call_head_step. apply call_head_step.
-    exists fn. repeat split; easy.
-  Qed.
+  Proof. apply language_mixin. Qed.
 
   Inductive rtc_step (p : prog Λ) : expr Λ → state Λ → expr Λ → state Λ → Prop :=
     rtc_refl e σ : rtc_step p e σ e σ
@@ -572,6 +238,15 @@ Section language.
   Definition safe p (e : expr Λ) (σ : state Λ) (Φ : val → Prop) := match to_val e with
     Some v => Φ v
   | None => reducible p e σ end.
+
+  Record pure_step (p : language.prog Λ) (e1 e2 : expr Λ) := {
+    pure_step_safe σ1 : reducible p e1 σ1;
+    pure_step_det σ1 e2' σ2 :
+      prim_step p e1 σ1 e2' σ2 → σ2 = σ1 ∧ e2' = e2
+  }.
+
+  Class PureExec (φ : Prop) (n : nat)  (p : language.prog Λ) (e1 e2 : expr Λ) :=
+    pure_exec : φ → relations.nsteps (pure_step p) n e1 e2.
 
 End language.
 
