theories/language/lifting.v
@@ -53,28 +53,6 @@ Proof.
   iApply wp_value; first done. iApply "H2".
 Qed.
 
-
-
-Lemma wp_lift_atomic_head_step {s E Φ} e1 :
-  to_val e1 = None →
-  (∀ σ1, state_interp σ1 ={E}=∗
-    ⌜head_reducible (penv_prog s) e1 σ1⌝ ∗
-    ▷ ∀ e2 σ2, ⌜head_step (penv_prog s) e1 σ1 e2 σ2⌝ ={E}=∗
-      state_interp σ2 ∗
-      from_option Φ False (to_val e2))
-  ⊢ WP e1 @ s; E {{ Φ }}.
-Proof.
-  iIntros (?) "H".
-  iApply (wp_lift_step_fupd s E _ e1)=>//; iIntros (σ1) "Hσ1".
-  iMod ("H" $! σ1 with "Hσ1") as "[%HH H]". iModIntro. iSplitR; first (iPureIntro; by eapply head_prim_reducible).
-  iIntros (e' σ' Hstep%head_reducible_prim_step). 2: {  destruct HH as (?&?&HH). do 2 eexists. done. }
-  do 2 iModIntro.
-  iMod ("H" $! e' σ' Hstep) as "[H1 H2]". iModIntro.
-  iFrame.
-  destruct (to_val e') eqn:?; last by iExFalso.
-  iApply wp_value; first done. iApply "H2".
-Qed.
-
 Lemma wp_lift_pure_det_step_no_fork `{!Inhabited (state Λ)} {s E Φ} e1 e2 :
   (∀ σ1, reducible (penv_prog s) e1 σ1) →
   (∀ σ1 e2' σ2, prim_step (penv_prog s) e1 σ1 e2' σ2 →
@@ -92,37 +70,15 @@ Proof.
   iFrame.
 Qed.
 
-  Record pure_step (p : language.prog Λ) (e1 e2 : expr Λ) := {
-    pure_step_safe σ1 : reducible p e1 σ1;
-    pure_step_det σ1 e2' σ2 :
-      prim_step p e1 σ1 e2' σ2 → σ2 = σ1 ∧ e2' = e2
-  }.
-
-  Record pure_head_step (p : language.prog Λ) (e1 e2 : expr Λ) := {
-    pure_head_step_safe σ1 : head_reducible p e1 σ1;
-    pure_head_step_det σ1 e2' σ2 :
-      head_step p e1 σ1 e2' σ2 → σ2 = σ1 ∧ e2' = e2
-  }.
-
-  Lemma pure_head_step_pure_step p e1 e2 : pure_head_step p e1 e2 -> pure_step p e1 e2.
-  Proof.
-    intros [Hp1 Hp2]. split.
-    - intros σ. destruct (Hp1 σ) as (e2' & σ2 & ?).
-      eexists e2', σ2. by apply head_prim_step.
-    - intros σ1 e2' σ2 ?%head_reducible_prim_step; eauto.
-  Qed.
-
-Class PureExec (φ : Prop) (n : nat)  (p : language.prog Λ) (e1 e2 : expr Λ) :=
-  pure_exec : φ → relations.nsteps (pure_step p) n e1 e2.
-
-Lemma pure_exec_fill φ n p e1 e2 K : PureExec φ n p  e1 e2 -> PureExec φ n p (fill K e1) (fill K e2).
+Lemma pure_exec_fill φ n p e1 e2 K : PureExec φ n p e1 e2 -> PureExec φ n p (fill K e1) (fill K e2).
 Proof.
   intros H Hφ. specialize (H Hφ). induction H as [|n x y z [Hred Hdet] Hstep IH]; econstructor.
   - econstructor.
     + intros σ1. destruct (Hred σ1) as (e' & σ' & H). do 2 eexists.
-      apply fill_prim_step, H.
-    + intros σ1 e2 σ2 (e2' & -> & HH)%fill_reducible_prim_step; last apply Hred.
-      destruct (Hdet _ _ _ HH) as (-> & ->); done.
+      apply prim_step_fill, H.
+    + intros σ1 e2 σ2 HH. apply fill_step_inv in HH as (?&?&HH).
+      2: { destruct (Hred σ1) as (?&?&?). by eapply val_stuck. }
+      apply Hdet in HH as (-> & ->). done.
   - apply IH.
 Qed.
 
