theories/ml_lang/lang_instantiation.v
@@ -10,148 +10,46 @@ Import ML_lang.
 
 Local Notation state := (gmap loc (option (list val))).
 
-Local Lemma fill_class (K : list ectx_item) (e:expr) :
-  is_Some (to_class_ML (fill K e)) → K = nil ∨ ∃ v, to_class_ML e = Some (ExprVal v).
-Proof.
-  intros [v Hv]. revert v Hv. induction K as [|k1 K] using rev_ind; intros v Hv. 1:now left. right.
-  rewrite fill_app in Hv.
-  destruct k1; cbn in Hv; try congruence.
-  + revert Hv. edestruct unmap_val eqn:Heq; try congruence.
-    intros H. injection H. intros <-. apply unmap_val_map in Heq.
-    assert (In (fill K e) (map Val l)) as [vv [Hvv' Hvv]]%in_map_iff.
-    1: rewrite Heq; apply in_app_iff; right; now left.
-    destruct (IHK (ExprVal vv)) as [Hl|Hr].
-    - rewrite <- Hvv'. easy.
-    - subst. cbn in *. subst. eexists. cbn. reflexivity.
-    - easy.
-Qed.
-
-Local Notation to_val e :=
-  (match to_class_ML e with Some (ExprVal v) => Some v | _ => None end).
-
-Local Lemma fill_val K e : is_Some (to_val (fill K e)) → is_Some (to_val e).
-Proof.
-  intros [? HH]. case_match; simplify_eq.
-  case_match; simplify_eq.
-  pose proof (mk_is_Some _ _ H) as H2.
-  apply fill_class in H2 as [->|[? ->]]; last done.
-  rewrite /= H //.
-Qed.
-
-Local Lemma fill_tail k K e e' :
-  to_val e = None →
-  to_val e' = None →
-  fill_item k e = fill K e' →
-   K = [] ∨ ∃ K', K = K' ++ [k] ∧ e = fill K' e'.
-Proof.
-  intros He He'.
-  destruct K.
-  + intros _. now left.
-  + destruct (@exists_last _ (e0::K)) as (L & l & Hl); first congruence.
-    rewrite Hl. unfold fill.
-    rewrite foldl_snoc. cbn. intros H. pose proof H as H_copy.
-    apply fill_item_no_val_inj in H_copy as ->.
-    2: easy. 
-    2: { destruct (to_val (foldl (flip fill_item) e' L)) eqn:Heq; last done.
-         edestruct (fill_val L e'). 1: eexists; apply Heq. congruence. }
-    right. eexists. split; first done. now apply fill_item_inj in H.
-Qed.
-
-Local Lemma of_to_val e v : to_val e = Some v → of_val v = e.
-Proof.
-  intros. eapply (of_to_class_ML e (ExprVal v)).
-  repeat case_match; by simplify_eq.
-Qed.
-
-Local Lemma to_val_extern fn vs :
-  to_val (Extern fn vs) = None.
-Proof.
-  repeat (case_match; simplify_eq; cbn in * ); eauto.
-Qed.
-
-Local Hint Resolve to_val_extern : core.
-
-Local Lemma fill_not_val K e : to_val e = None → to_val (fill K e) = None.
-Proof.
-  intros HH. destruct (to_val (fill K e)) eqn:Heq; try done.
-  destruct (fill_val K e); try done. congruence.
-Qed.
-
-Local Lemma fill_comp_item k K e : fill (k :: K) e = fill K (fill_item k e).
-Proof. reflexivity. Qed.
-
-Local Lemma fill_inj K : Inj (=) (=) (fill K).
-Proof.
-  intros e1 e2.
-  induction K as [|Ki K IH] in e1, e2 |- *; rewrite /Inj; first done.
-  rewrite !fill_comp_item. by intros ?%IH%fill_item_inj.
-Qed.
-
-Local Lemma fill_ctx K s vv K' e :
-  fill K' e = fill K (of_class_ML (ExprCall s vv)) →
-  (∃ v, e = Val v) ∨ (∃ K2, K = K2 ++ K').
-Proof. cbn.
-  induction K' as [|[] K' IH] in K,e|-*; intros H; first last.
-  1-22: destruct  (IH _ _ H) as [(v & Hv)|(K2 & ->)]; try (cbn in *; congruence).
-  1-22:  destruct (to_val e) eqn:Heq; first (apply of_to_val in Heq; by left; eexists).
-  1-22:  rewrite fill_comp_item in H.
-  1-22:  rewrite fill_app in H; apply fill_inj in H.
-  1-22:  apply fill_tail in H as H2; try (simplify_eq; eauto; congruence).
-  1-22:  destruct H2 as [->|(K3 & -> & HK3)]; try (cbn in *; congruence).
-  1-24:  try (right; exists K3; by rewrite <- app_assoc).
-  - exfalso. cbn in H. assert (In e (map Val vv)) as Hin.
-    + assert (map Val va ++ e :: ve = map Val vv) as <- by congruence.
-      apply in_app_iff. right. now left.
-    + apply in_map_iff in Hin. destruct Hin as (v & Hv & Hin). rewrite <- Hv in Heq. cbn in Heq. congruence.
-  - cbn. right. eexists. by erewrite app_nil_r.
-Qed.
-
-Lemma melocoton_lang_mixin_ML :
+Local Lemma melocoton_lang_mixin_ML :
   @LanguageMixin expr val ml_function (list ectx_item) state
-                 of_class_ML to_class_ML
+                 of_val lang.ML_lang.to_val lang.ML_lang.of_call lang.ML_lang.is_call
                  nil comp_ectx fill
-                 apply_function head_step.
+                 apply_function prim_step.
 Proof. split.
-  + apply to_of_class_ML.
-  + apply of_to_class_ML.
-  + intros *; inversion 1.
-  + intros p f vs σ1 e2 σ2. split.
-    - intros H. inversion H; subst. inversion H; subst.
-      repeat econstructor; [apply H2|]. simplify_eq. congruence.
-    - intros ([args ee] & H1 & H2 & ->). econstructor; eauto.
-  + intros K K' e s' vv Heq.
-    destruct (fill_ctx K' s' vv K e) as [(v&HL)|(K2&HK2)].
-    - apply Heq.
-    - right. exists v. rewrite HL. easy.
-    - left. exists K2. easy.
-  + intros p1 p2 e1 σ1 e2 σ2 H Hnc.
-    inversion H; subst. all: try by econstructor.
-    cbn in Hnc. rewrite map_unmap_val in Hnc. congruence.
+  + apply lang.ML_lang.to_of_val.
+  + apply lang.ML_lang.of_to_val.
+  + apply lang.ML_lang.val_prim_step.
+  + apply lang.ML_lang.call_prim_step.
+  + apply lang.ML_lang.prim_step_call_dec.
+  + apply lang.ML_lang.prim_step_no_call.
+  + apply lang.ML_lang.is_val_not_call.
+  + apply lang.ML_lang.is_call_in_cont.
   + done.
-  + intros e; rewrite /comp_ectx app_nil_r //.
-  + now intros e.
-  + intros K1 K2 e. rewrite fill_app //.
-  + intros K a b. apply fill_inj.
-  + apply fill_class.
-  + intros p.
-    intros K K' e1 e1' σ1 e2 σ2 Hfill Hred Hstep; revert K' Hfill.
-    induction K as [|Ki K IH] using rev_ind=> /= K' Hfill; eauto using app_nil_r.
-    destruct K' as [|Ki' K' _] using @rev_ind; simplify_eq/=.
-    { rewrite fill_app in Hstep. apply head_ctx_step_val in Hstep.
-      apply fill_val in Hstep. destruct Hstep as [? Hstep].
-      by repeat (case_match; simplify_eq). }
-    rewrite !fill_app /= in Hfill.
-    assert (Ki = Ki') as ->.
-    { eapply fill_item_no_val_inj, Hfill.
-      2: { by eapply val_head_stuck, fill_not_val in Hstep. }
-      eapply fill_not_val. by destruct e1. }
-    simplify_eq. destruct (IH K') as [K'' ->]; auto.
-    exists K''. rewrite /comp_ectx assoc //.
-  + intros p K e σ1 e2 σ2.
-    destruct K as [|Ki K _] using rev_ind; simpl; first by auto.
-    rewrite fill_app /=.
-    intros [v' ?]%head_ctx_step_val%fill_val. right. exists v'.
-    by repeat (case_match; simplify_eq).
+  + done.
+  + apply lang.ML_lang.is_call_of_call_inv.
+  + intros *. eapply lang.ML_lang.fill_val.
+  + eapply lang.ML_lang.fill_comp.
+  + done.
+  + eapply lang.ML_lang.prim_step_fill.
+  + intros *. eapply lang.ML_lang.fill_step_inv.
 Qed.
 
 Canonical Structure ML_lang := Language melocoton_lang_mixin_ML.
+
+Record pure_head_step (p : gmap _ _) (e1 e2 : expr) := {
+  pure_head_step_safe σ1 : head_reducible p e1 σ1;
+  pure_head_step_det σ1 e2' σ2 :
+    head_step p e1 σ1 e2' σ2 → σ2 = σ1 ∧ e2' = e2
+}.
+
+Lemma pure_head_step_pure_step p e1 e2 :
+  pure_head_step p e1 e2 → pure_step p e1 e2.
+Proof.
+  intros [Hp1 Hp2]. split.
+  - intros σ. destruct (Hp1 σ) as (e2' & σ2 & ?).
+    eexists e2', σ2. by apply head_prim_step.
+  - intros σ1 e2' σ2 ?%head_reducible_prim_step; eauto.
+Qed.
+
+Lemma head_prim_reducible p e σ : head_reducible p e σ → reducible p e σ.
+Proof. intros (e'&σ'&?). eexists e', σ'. by apply head_prim_step. Qed.
