theories/ml_lang/primitive_laws.v
@@ -117,7 +117,7 @@ Lemma mapsto_combine l dq1 dq2 v1 v2 :
 Proof.
   iIntros "Hl1 Hl2". iDestruct (mapsto_combine with "Hl1 Hl2") as "[$ Heq]".
   by iDestruct "Heq" as %[= ->].
-Qed. 
+Qed.
 
 Lemma mapsto_frac_ne l1 l2 dq1 dq2 v1 v2 :
   ¬ ✓(dq1 ⋅ dq2) → l1 ↦M{dq1} v1 -∗ l2 ↦M{dq2} v2 -∗ ⌜l1 ≠ l2⌝.
@@ -127,6 +127,26 @@ Proof. apply mapsto_ne. Qed.
 
 Lemma mapsto_persist l dq v : l ↦M{dq} v ==∗ l ↦M□ v.
 Proof. apply mapsto_persist. Qed.
+
+Lemma wp_lift_atomic_head_step {s E Φ} e1 :
+  to_val e1 = None →
+  (∀ σ1, state_interp σ1 ={E}=∗
+    ⌜head_reducible (penv_prog s) e1 σ1⌝ ∗
+    ▷ ∀ e2 σ2, ⌜head_step (penv_prog s) e1 σ1 e2 σ2⌝ ={E}=∗
+      state_interp σ2 ∗
+      from_option Φ False (to_val e2))
+  ⊢ WP e1 @ s; E {{ Φ }}.
+Proof.
+  iIntros (?) "H".
+  iApply (wp_lift_step_fupd s E _ e1)=>//; iIntros (σ1) "Hσ1".
+  iMod ("H" $! σ1 with "Hσ1") as "[%HH H]". iModIntro. iSplitR; first (iPureIntro; by eapply head_prim_reducible).
+  iIntros (e' σ' Hstep%head_reducible_prim_step). 2: {  destruct HH as (?&?&HH). do 2 eexists. done. }
+  do 2 iModIntro.
+  iMod ("H" $! e' σ' Hstep) as "[H1 H2]". iModIntro.
+  iFrame.
+  destruct (to_val e') eqn:?; last by iExFalso.
+  iApply wp_value; first done. iApply "H2".
+Qed.
 
 Lemma wp_allocN pe E v n :
   (0 ≤ n)%Z →
