theories/ml_lang/proofmode.v
@@ -177,6 +177,7 @@ Tactic Notation "wp_extern" :=
   lazymatch goal with
   | |- envs_entails _ (wp ?s ?E ?e ?Q) =>
     let e := eval simpl in e in
+    let e := eval unfold lang.ML_lang.of_call in e in
     reshape_expr e ltac:(fun K e' => match e' with Extern (?s) (map Val ?vv) => 
       iApply (@wp_extern _ _ ML_lang _ _ _ K _ s vv); [try (iPureIntro; vm_compute; reflexivity) | ] end)
     || fail "wp_extern: expression not a call"
